Cslib/Computability/LambdaCalculus/LocallyNameless/Fsub/Properties.lean
@@ -24,14 +24,17 @@ variable {Var : Type u} [HasFresh Var] [DecidableEq Var]
 
 namespace LambdaCalculus.LocallyNameless.Fsub
 
-omit [HasFresh Var] [DecidableEq Var] in
- /-- An opening appearing in both sides of an equality of terms can be removed. -/
-@[grind]
-lemma Ty.open_lc_aux (T : Ty Var) j V i U (neq : i ≠ j) (h : T⟦j ↝ V⟧ = (T⟦j ↝ V⟧)⟦i ↝ U⟧) : 
-    T = T⟦i ↝ U⟧ := by induction T generalizing j i <;> grind
+open Ty Term
 
-@[grind]
-lemma Ty.open_lc (T : Ty Var) U k (lc : T.LC) : T = T⟦k ↝ U⟧ := by
+omit [HasFresh Var] [DecidableEq Var] in
+/-- An opening appearing in both sides of an equality of terms can be removed. -/
+@[scoped grind]
+lemma Ty.openRec_lc_aux (T : Ty Var) j V i U (neq : i ≠ j) (h : T⟦j ↝ V⟧ᵞ = T⟦j ↝ V⟧ᵞ⟦i ↝ U⟧ᵞ) : 
+    T = T⟦i ↝ U⟧ᵞ := by induction T generalizing j i <;> grind
+
+/-- A locally closed type is unchanged by opening. -/
+@[scoped grind =_]
+lemma Ty.openRec_lc (T : Ty Var) U k (lc : T.LC) : T = T⟦k ↝ U⟧ᵞ := by
   induction lc generalizing k
   case all => 
     -- TODO: how to tell grind to try `free_union`?
@@ -41,72 +44,65 @@ lemma Ty.open_lc (T : Ty Var) U k (lc : T.LC) : T = T⟦k ↝ U⟧ := by
 
 omit [HasFresh Var] in
 /-- Substitution of a free variable not present in a type leaves it unchanged. -/
+@[scoped grind]
 lemma Ty.subst_fresh (Z : Var) (U T : Ty Var) (nmem : Z ∉ T.fv) : T = T[Z := U] := by
   induction T <;> grind
 
 /-- Substitution of a locally closed type distributes with opening. -/
 lemma Ty.subst_openRec (T1 T2 : Ty Var) (X : Var) (P : Ty Var) k (lc : P.LC) : 
-    (T1⟦k ↝ T2⟧)[X := P] = (T1[X := P])⟦k ↝ T2[X := P]⟧ := by
+    (T1⟦k ↝ T2⟧ᵞ)[X := P] = T1[X := P]⟦k ↝ T2[X := P]⟧ᵞ := by
   induction T1 generalizing k <;> grind
 
 /-- Specialize `Ty.subst_openRec` to the first opening. -/
 lemma Ty.subst_open (T1 T2 : Ty Var) (X : Var) (P : Ty Var) (lc : P.LC) :
-    (T1 ^ T2)[X := P] = T1[X := P] ^ T2[X := P] := subst_openRec _ _ _ _ _ lc
+    (T1 ^ᵞ T2)[X := P] = T1[X := P] ^ᵞ T2[X := P] := subst_openRec _ _ _ _ _ lc
 
 /-- Specialize `Ty.subst_open` to free variables. -/
 lemma Ty.subst_open_var (X Y : Var) (P T : Ty Var) (neq : Y ≠ X) (lc : P.LC) :
-    (T[X := P]) ^ fvar Y = (T ^ fvar Y)[X := P] := by
+    (T[X := P]) ^ᵞ fvar Y = (T ^ᵞ fvar Y)[X := P] := by
   have := Ty.subst_open T (fvar Y) X P lc
   grind
 
 omit [HasFresh Var] in
 /-- Opening to a type is equivalent to opening to a free variable and substituting. -/
 lemma Ty.openRec_subst_intro (X : Var) (T2 U : Ty Var) (k : ℕ) (nmem : X ∉ T2.fv) :
-    T2⟦k ↝ U⟧ = (T2⟦k ↝ fvar X⟧)[X := U] := by
+    T2⟦k ↝ U⟧ᵞ = (T2⟦k ↝ fvar X⟧ᵞ)[X := U] := by
   induction T2 generalizing U k <;> grind
 
 omit [HasFresh Var] in
 /-- Specialize `Ty.openRec_subst_intro` to the first opening. -/
 lemma Ty.open_subst_intro (X : Var) (T2 U : Ty Var) (nmem : X ∉ T2.fv) :
-    T2 ^ U = (T2 ^ fvar X)[X := U] := by
-  apply openRec_subst_intro
-  grind
+    T2 ^ᵞ U = (T2 ^ᵞ fvar X)[X := U] := openRec_subst_intro _ _ _ _ nmem
 
--- TODO: if I make this local, it fails...
 omit [HasFresh Var] [DecidableEq Var] in
---@[local grind =>]
-@[grind =>]
+@[scoped grind]
 lemma Term.openRec_ty_lc_aux₁ (e : Term Var) j (u : Term Var) i (P : Ty Var) 
-    (eq : e⟦j ↝ u⟧ = e⟦j ↝ u⟧⟦i ↝ P⟧) : e = e⟦i ↝ P⟧
+    (eq : e⟦j ↝ u⟧ᵗᵗ = e⟦j ↝ u⟧ᵗᵗ⟦i ↝ P⟧ᵗᵞ) : e = e⟦i ↝ P⟧ᵗᵞ
   := by induction e generalizing j i <;> grind
 
 omit [HasFresh Var] [DecidableEq Var] in
-@[local grind]
-lemma Term.openRec_ty_lc_aux₂ (e : Term Var) j (Q : Term Var) i (P : Ty Var) : 
-    i ≠ j → e⟦j ↝ Q⟧ = e⟦j ↝ Q⟧⟦i ↝ P⟧ → e = e⟦i ↝ P⟧ := by
-  induction e <;> grind 
+@[scoped grind]
+lemma Term.openRec_ty_lc_aux₂ (e : Term Var) j (Q : Ty Var) i (P : Ty Var) : 
+    i ≠ j → e⟦j ↝ Q⟧ᵗᵞ = e⟦j ↝ Q⟧ᵗᵞ⟦i ↝ P⟧ᵗᵞ → e = e⟦i ↝ P⟧ᵗᵞ := by
+  induction e generalizing j i <;> grind
 
-lemma Term.openRec_ty_lc (e : Term Var) (U : Ty Var) k (e_lc : e.LC) : e = e⟦k ↝ U⟧ := by
+lemma Term.openRec_ty_lc (e : Term Var) (U : Ty Var) k (e_lc : e.LC) : e = e⟦k ↝ U⟧ᵗᵞ := by
   induction e generalizing k
   case abs T t ih =>
     simp [openRec_ty]
     refine ⟨by grind, ?_⟩
     cases e_lc with | abs L T_lc cofin =>
     have ⟨x, free⟩ := fresh_exists L
-    --rw [←openRec_ty_lc_aux₁ (j := 0) (u := fvar x)]
-    --rw [←openRec_ty_lc_aux₂ (j := 0) (Q := fvar x)]
+    ----rw [←openRec_ty_lc_aux₁ (j := 0) (u := fvar x)]
+    ----rw [←openRec_ty_lc_aux₂ (j := 0) (Q := fvar x)]
     sorry    
   case tabs => sorry
   case let' => sorry
   case case => sorry
   all_goals grind
 
+omit [HasFresh Var] in
 lemma Term.subst_ty_fresh (X : Var) (U : Ty Var) (e : Term Var) (nmem : X ∉ e.fv_ty) : 
-    e = e [X := U] := by
-  induction e
-  case fvar X' =>
-    -- TODO: make grind do this... something with notation?? a grind I missed???
-    rfl
-  all_goals grind [Ty.subst_fresh]
+    e = e [X := U] := by induction e <;> grind
 
 end LambdaCalculus.LocallyNameless.Fsub
